General invariant tactic.

theories/proofmode/classes.v
@@ -1,4 +1,5 @@
 From iris.bi Require Export bi.
+From stdpp Require Import namespaces.
 Set Default Proof Using "Type".
 Import bi.
 
@@ -466,6 +467,31 @@ Lemma as_valid_1 (φ : Prop) {PROP : bi} (P : PROP) `{!AsValid φ P} : φ → P.
 Proof. by apply as_valid. Qed.
 Lemma as_valid_2 (φ : Prop) {PROP : bi} (P : PROP) `{!AsValid φ P} : P → φ.
 Proof. by apply as_valid. Qed.
+
+(* Input: `P`; Outputs: `N`,
+   Extracts the namespace associated with an invariant assertion. Used for `iInv`. *)
+Class IntoInv {PROP : bi} (P: PROP) (N: namespace).
+Arguments IntoInv {_} _%I _.
+Hint Mode IntoInv + ! - : typeclass_instances.
+
+(* Input: `Pinv`;
+   - `Pinv`, an invariant assertion
+   - `Ps_aux` is a list of additional assertions needed for opening an invariant;
+   - `Pout` is the assertion obtained by opening the invariant;
+   - `Q` is a goal on which iInv may be invoked;
+   - `Q'` is the transformed goal that must be proved after opening the invariant.
+
+   There are similarities to the definition of ElimModal, however we
+   want to be general enough to support uses in settings where there
+   is not a clearly associated instance of ElimModal of the right form
+   (e.g. to handle Iris 2.0 usage of iInv).
+*)
+Class ElimInv {PROP : bi} (φ: Prop) (N: namespace)
+      (Pinv : PROP) (Ps_aux: list PROP) (Pout Q Q': PROP) :=
+  elim_inv : φ → Pinv ∗ [∗] Ps_aux ∗ (Pout -∗ Q') ⊢ Q.
+Arguments ElimInv {_} _ _ _  _%I _%I _%I _%I : simpl never.
+Arguments elim_inv {_} _ _ _%I _%I _%I _%I _%I _%I.
+Hint Mode ElimInv + - - ! - - - - : typeclass_instances.
 
 (* We make sure that tactics that perform actions on *specific* hypotheses or
 parts of the goal look through the [tc_opaque] connective, which is used to make
