theories/proofmode/coq_tactics.v
@@ -209,6 +209,16 @@ Proof.
   repeat apply sep_mono=>//; apply affinely_persistently_if_flag_mono; by destruct q1.
 Qed.
 
+Lemma envs_lookup_delete_list_cons Δ Δ' Δ'' rp j js p1 p2 P Ps :
+  envs_lookup_delete rp j Δ = Some (p1, P, Δ') →
+  envs_lookup_delete_list rp js Δ' = Some (p2, Ps, Δ'') →
+  envs_lookup_delete_list rp (j :: js) Δ = Some (p1 && p2, (P :: Ps), Δ'').
+Proof. rewrite //= => -> //= -> //=. Qed.
+
+Lemma envs_lookup_delete_list_nil Δ rp :
+  envs_lookup_delete_list rp [] Δ = Some (true, [], Δ).
+Proof. done. Qed.
+
 Lemma envs_lookup_snoc Δ i p P :
   envs_lookup i Δ = None → envs_lookup i (envs_snoc Δ p i P) = Some (p, P).
 Proof.
@@ -1158,6 +1168,20 @@ Lemma tac_modal_elim Δ Δ' i p φ P' P Q Q' :
 Proof.
   rewrite envs_entails_eq => ???? HΔ. rewrite envs_replace_singleton_sound //=.
   rewrite HΔ affinely_persistently_if_elim. by eapply elim_modal.
+Qed.
+
+(** * Invariants *)
+Lemma tac_inv_elim Δ1 Δ2 Δ3 js j p φ N P' P Ps Q Q' :
+  envs_lookup_delete_list false js Δ1 = Some (p, P :: Ps, Δ2) →
+  ElimInv φ N P Ps P' Q Q' →
+  φ →
+  envs_app false (Esnoc Enil j P') Δ2 = Some Δ3 →
+  envs_entails Δ3 Q' → envs_entails Δ1 Q.
+Proof.
+  rewrite envs_entails_eq => ???? HΔ. rewrite envs_lookup_delete_list_sound //.
+  rewrite envs_app_singleton_sound //=.
+  rewrite HΔ //= affinely_persistently_if_elim //=.
+  rewrite -sep_assoc. by eapply elim_inv.
 Qed.
 End bi_tactics.
 
